concurrency/verif_bst_conc_nblocking.v
@@ -30,6 +30,8 @@ Proof.
 Qed.
 Hint Resolve node_data_saturate_local: saturate_local.
 
+Definition node_data_without_value (info: option ghost_info) g  tp lp rp  (range:number * number)  :=  
+(match info with Some data =>  EX sh, !!(readable_share sh /\ Int.min_signed <= data.1.1.1 <= Int.max_signed/\ is_pointer_or_null lp /\ is_pointer_or_null rp /\ is_pointer_or_null data.1.1.2) &&  data_at sh t_struct_tree (Vint (Int.repr data.1.1.1),(data.1.1.2,(lp,rp))) tp * in_tree  data.1.2 ( fst range, Finite_Integer (data.1.1.1)) lp g * in_tree data.2 ( Finite_Integer (data.1.1.1), snd range) rp g | None => !!(tp = nullval /\ lp = nullval /\ rp = nullval) && emp end).
 
 
 
@@ -41,9 +43,16 @@ SEP ( |>P; AS && cored;in_tree g_current (n1,n2) np g; mem_mgr gv; malloc_token 
    nodebox_rep sh b g_root g 
    ))%assert.
    
+Definition lookup_inv (b: val)  (sh: share) (x: Z) ( g_root:gname) gv (g:gname)  (inv_names : invG) (P:mpred) (AS:mpred) Q : environ -> mpred :=
+  (EX nb:val, EX tp1: val, EX g_current:gname,
+   PROP ( )
+   LOCAL (temp _p tp1; temp _ap b; temp _t b; temp _x (vint x); gvars gv)
+   SEP ((if eq_dec tp1 nullval
+        then Q nullval
+        else(EX n1:number, EX n2:number, EX n5:number, EX n6:number,  EX info : option ghost_info, EX lp:val, EX rp:val,!! (check_key_exist' x (n1, n2) = true/\ range_inclusion (n5,n6) (n1,n2)=true) && |> P* ghost_snap (n1, n2, info) g_current * node_data_without_value info g tp1 lp rp (n1, n2)*
+      in_tree g_current ( n5, n6) nb g* (AS && cored ))) * mem_mgr gv * nodebox_rep sh b g_root g))%assert.
    
-Definition node_data_without_value (info: option ghost_info) g  tp lp rp  (range:number * number)  :=  
-(match info with Some data =>  EX sh, !!(readable_share sh /\ Int.min_signed <= data.1.1.1 <= Int.max_signed/\ is_pointer_or_null lp /\ is_pointer_or_null rp /\ is_pointer_or_null data.1.1.2) &&  data_at sh t_struct_tree (Vint (Int.repr data.1.1.1),(data.1.1.2,(lp,rp))) tp * in_tree  data.1.2 ( fst range, Finite_Integer (data.1.1.1)) lp g * in_tree data.2 ( Finite_Integer (data.1.1.1), snd range) rp g | None => !!(tp = nullval /\ lp = nullval /\ rp = nullval) && emp end).
+   
 
 Lemma node_data_without_value_R: forall (info: option ghost_info) g  tp lp rp  (range:number *number),  node_data_without_value info g tp  lp rp  range |-- if (eq_dec tp nullval) then !!(info = None /\ lp = nullval /\ rp = nullval) && emp  else 
 EX data, EX sh, !!(readable_share sh/\ info = Some data  /\ Int.min_signed <= data.1.1.1 <= Int.max_signed/\ is_pointer_or_null lp /\ is_pointer_or_null rp /\  is_pointer_or_null data.1.1.2) &&   data_at sh t_struct_tree (Vint (Int.repr data.1.1.1),(data.1.1.2,(lp,rp))) tp * in_tree data.1.2( fst range, Finite_Integer data.1.1.1) lp g * in_tree data.2 ( Finite_Integer data.1.1.1, snd range) rp g.
@@ -69,7 +78,286 @@ Proof.
 Qed.
 Hint Resolve node_data_without_value_saturate_local: saturate_local.
 
-
+Lemma body_lookup: semax_body Vprog Gprog f_lookup lookup_spec.
+Proof.
+start_function.
+unfold atomic_shift. Intros P.
+set (AS := ashift _ _ _ _ _ _).
+unfold nodebox_rep. Intros tp lp.
+forward. (* atom_ptr *ap = t *)
+sep_apply cored_dup.
+sep_apply in_tree_split. 
+focus_SEP 2.
+(* struct tree *p = atomic_load_ptr(ap) *)
+forward_call (b, top, empty, fun tp : val => if eq_dec tp nullval then  Q nullval else |> P * EX n n0:number, EX lp:val, EX rp:val, EX info: option ghost_info, !!(range_inclusion (Neg_Infinity, Pos_Infinity) (n, n0) = true) && ghost_snap (n, n0,info) g_root * node_data_without_value info g tp lp rp  (n,n0) , inv_names).
+    { subst Frame;instantiate (1 := [AS && cored;in_tree g_root (Neg_Infinity, Pos_Infinity) b g; mem_mgr gv;iter_sepcon (λ p : val, EX sh1 : share, data_at_ sh1 t_struct_tree p) lp;bst_conc_nblocking_spec.atomic_ptr_at sh tp b]).  simpl;cancel.
+      iIntros "((in & [AS1 _]) & P )". 
+      iMod ("AS1" with "P") as (BST) "[Tree Tclose]". 
+      iDestruct "Tree" as "(% & Tree)".
+      unfold tree_rep2 at 1.
+      iDestruct "Tree" as (tg) "((% & Tree) & gref)".
+      iPoseProof (node_exist_in_tree with "[gref in]") as "%". iFrame. destruct H2 as [r H2]. destruct r as [n n0]. destruct H2.
+      iPoseProof ( extract_left_node_info_from_ghost_tree_rep with "Tree") as "Hadd". apply H2. intros. simpl;auto.
+      iDestruct "Hadd" as ( tp1 o lp1 rp1 v0) "(info & Tree)". 
+      unfold node_information at 1.
+      iDestruct "info" as "( % &  ((p & master) & info))". 
+       iModIntro; iExists Ews, tp1. iFrame "p".
+       iSplitL ""; [iSplit; auto; iPureIntro; split; auto; tauto|].
+        iIntros "p".
+        iPoseProof (make_snap with "[master]") as "master". iFrame.
+        iMod ("master") as "[snap master]".  
+        iDestruct "in" as (sh2) "in".
+       iMod (own_dealloc with "in") as "_". rewrite node_data_R.
+       destruct (eq_dec tp1 nullval).
+       * iMod (own_dealloc with "snap") as "_".
+         iDestruct "Tclose" as "[_ Tclose]".  iSpecialize ("Tclose" $! nullval). iApply "Tclose". iDestruct "info" as "(% & _)".
+         rewrite prop_true_andp.
+         unfold tree_rep2.
+          rewrite -> exp_sepcon1.  
+         iExists tg.
+         iFrame;iSplit;auto.
+         iApply "Tree".
+         unfold node_information, node_data. destruct H5. rewrite H5. iFrame. iPureIntro. split;auto.
+         split;auto. symmetry. apply lookup_not_in. rewrite <- H1 in H0. destruct H5;destruct H6;destruct H7.  rewrite H5 in H4.  rewrite H8 in H4. eapply range_info_in_tree_not_In in H4.  rewrite <- H1. apply H4. auto. 
+         assert ( n= Neg_Infinity /\ n0 = Pos_Infinity).
+       { unfold range_inclusion in H3. apply andb_prop in H3. destruct H3. destruct n;destruct n0;simpl in H3,H9. discriminate. discriminate. discriminate. discriminate. discriminate. auto. discriminate. discriminate. discriminate. }
+        destruct H9; subst n n0;simpl;auto. intros. simpl;auto.
+        *        
+        iDestruct "Tclose" as "[Tclose _]". unfold node_data_without_value.
+       iDestruct "info" as (g0 sh1) "info".  destruct g0 as [[[k v3] g1 ] g2].  iDestruct "info" as "(((((% & v) & malloc ) & tp) & g1) & g2)". simpl in *.
+         destruct H5. apply split_readable_share in H5. destruct H5 as (sh3 & sh4 & H7 & H9 & H10). rewrite <- (data_at_share_join sh3 sh4 sh1 _ _ _). iDestruct "tp" as "(tp1 & tp2)".
+          rewrite (in_tree_split g1 ( n, Finite_Integer k) lp1 g). rewrite ( in_tree_split g2 ( Finite_Integer k, n0) rp1 g ). iDestruct "g1" as "(g11 & g12)". iDestruct "g2" as "(g21 & g22)".
+        rewrite -> exp_sepcon2.  iExists n.  rewrite -> exp_sepcon2.  iExists n0.  rewrite -> exp_sepcon2.  iExists lp1. rewrite -> exp_sepcon2. iExists rp1. rewrite -> exp_sepcon2. iExists (Some (k,v3,g1,g2)). simpl. 
+        rewrite <- !sepcon_assoc.   rewrite -> exp_sepcon2. iExists sh3. rewrite (prop_true_andp _ (ghost_snap (n, n0, Some (k, v3, g1, g2)) g_root)). 
+        rewrite (prop_true_andp ( readable_share sh3 ∧ (Int.min_signed ≤ k ∧ k ≤ Int.max_signed)∧ is_pointer_or_null lp1 ∧ is_pointer_or_null rp1 /\  is_pointer_or_null v3  ) _ ). destruct H6. rewrite H5.
+        iFrame .
+       iApply "Tclose". 
+       iFrame.
+       iSplit. iPureIntro;auto.
+       unfold tree_rep2.
+       iExists tg.
+       iFrame;iSplit;auto.
+       iApply "Tree".
+       unfold node_information, node_data. rewrite -> exp_sepcon2.  iExists sh4.
+       iFrame. iSplit. iPureIntro;auto. auto. destruct H6; split; auto. auto. auto.
+      
+  }
+  Intros tp1.
+  forward_while (lookup_inv b sh x g_root gv g inv_names P AS Q). 
+ * (* Precondition *) 
+    unfold lookup_inv. Exists b tp1 g_root. unfold nodebox_rep.  destruct (eq_dec tp1 nullval).  Exists tp lp. entailer!. admit.  (* extra AS && cored, need to fix*)
+    Intros n0 n1 lp0 rp info. Exists n0 n1 Neg_Infinity Pos_Infinity info lp0 rp. Exists tp lp. sep_apply in_tree_split. 
+    assert ( n0= Neg_Infinity /\ n1 = Pos_Infinity).
+       { unfold range_inclusion in H0. apply andb_prop in H0. destruct H0. destruct n0;destruct n1;simpl in H0,H1. discriminate. discriminate. discriminate. discriminate. discriminate. auto. discriminate. discriminate. discriminate. }
+   destruct H1. subst n0. subst n1.  entailer!.
+ * (* type checking *) 
+    destruct (eq_dec tp0 nullval);Intros. entailer!. Intros n1 n2 n5 n6 info lp0 rp. entailer!.
+ 
+ * (*Loop Body *)
+  Intros.  if_tac. contradiction HRE.
+  Intros n1 n2 n5 n6 info lp1 rp .
+  sep_apply node_data_without_value_R. destruct (eq_dec tp0 nullval). contradiction HRE. Intros data sh1.
+  destruct data as [[[k vp] g1 ] g2]. simpl. 
+  forward. simpl in H5.  
+  forward_if; [ | forward_if ].
+   **  (* first if, then clause: x<y *)   
+    forward.
+    sep_apply (in_tree_split g1 (n1, Finite_Integer k) lp1 g).
+    sep_apply cored_dup.
+    forward_call (lp1, top, empty, fun tp : val => if eq_dec tp nullval then  Q nullval else |> P * EX n n0:number, EX lp:val, EX rp:val, EX info: option ghost_info, !!(range_inclusion (n1, Finite_Integer k) (n,n0) = true) && ghost_snap (n, n0,info) g1 * node_data_without_value info g tp lp rp  (n,n0) , inv_names).
+    { subst Frame;instantiate (1 := [ AS && cored ; in_tree g1 (n1, Finite_Integer k) lp1 g; mem_mgr gv; data_at sh1 t_struct_tree (vint k, (vp, (lp1, rp))) tp0; nodebox_rep sh b g_root g]).  simpl;cancel.
+      iIntros "((((( [AS1 _] & in1) & in2) & P ) & snap) & in)". 
+      iMod ("AS1" with "P") as (BST) "[Tree Tclose]". 
+      iDestruct "Tree" as "(% & Tree)".
+      unfold tree_rep2 at 1.
+      iDestruct "Tree" as (tg) "((% & Tree) & gref)".
+      iPoseProof (node_exist_in_tree with "[gref in1]") as "%". iFrame. destruct H10 as [r H10]. destruct r as [n3 n4]. destruct H10.
+      iPoseProof ( extract_left_node_info_from_ghost_tree_rep with "Tree") as "Hadd". apply H10. intros. simpl;auto.
+      iDestruct "Hadd" as ( tp2 o lp2 rp2 v) "(info & Tree)". 
+      unfold node_information at 1.
+      iDestruct "info" as "(% &((p & master) & info))". 
+       iModIntro; iExists Ews, tp2. iFrame "p".
+       iSplitL ""; [iSplit; auto; iPureIntro; split; auto; tauto|].
+        iIntros "p".
+        iPoseProof (make_snap with "[master]") as "master". iFrame.
+        iMod ("master") as "[snap1 master]". 
+        iDestruct "in" as (sh7) "in".
+       iMod (own_dealloc with "in") as "_".
+       iDestruct "in1" as (sh8) "in1".
+       iMod (own_dealloc with "in1") as "_". 
+        iDestruct "in2" as (sh2) "in2".
+       iMod (own_dealloc with "in2") as "_".
+        iMod (own_dealloc with "snap") as "_".
+       rewrite  node_data_R. unfold node_data_without_value. 
+       assert ( check_key_exist' x (n3,n4) = true).
+       { unfold check_key_exist', range_inclusion in *. apply andb_true_intro. apply andb_prop in H1. apply andb_prop in H11. destruct H1, H11. split.
+          apply less_than_equal_less_than_transitivity with (b := n1);auto. apply less_than_less_than_equal_transitivity with  (b := Finite_Integer k);auto. simpl. apply Zaux.Zlt_bool_true ;auto.
+        }  
+       destruct (eq_dec tp2 nullval).
+       * iMod (own_dealloc with "snap1") as "_". iDestruct "Tclose" as "[_ Tclose]".
+         iSpecialize ("Tclose" $! nullval). iApply "Tclose". iDestruct "info" as "(% & _)".
+         rewrite prop_true_andp.
+         unfold tree_rep2.
+          rewrite -> exp_sepcon1.  
+         iExists tg.
+         iFrame;iSplit;auto.
+         iApply "Tree".
+         unfold node_information, node_data. destruct H14. rewrite H14. iFrame. iPureIntro. split;auto.
+         split;auto. symmetry. apply lookup_not_in. destruct H14. rewrite  H14 in H12. destruct H15. destruct H16.  rewrite H17 in H12.  eapply range_info_in_tree_not_In in H12.  rewrite <- H9. apply H12. rewrite <-H9 in H8;auto. auto. intros;auto. 
+        * 
+          iDestruct "Tclose" as "[Tclose _]".    iDestruct "info" as (g0 sh3) "info".  destruct g0 as [[[k1 v3] g11 ] g12].  iDestruct "info" as "(((((% & v) & malloc ) & tp) & g1) & g2)". simpl in *.
+         destruct H14. apply split_readable_share in H14. destruct H14 as (sh4 & sh5 & H18 & H17 & H16). rewrite <- (data_at_share_join sh4 sh5 sh3 _ _ _). iDestruct "tp" as "(tp1 & tp2)".
+          rewrite (in_tree_split g11 ( n3, Finite_Integer k1) lp2 g). rewrite ( in_tree_split g12 ( Finite_Integer k1, n4) rp2 g ). iDestruct "g1" as "(g11 & g12)". iDestruct "g2" as "(g21 & g22)".
+        rewrite -> exp_sepcon2.  iExists n3.  rewrite -> exp_sepcon2.  iExists n4.  rewrite -> exp_sepcon2.  iExists lp2. rewrite -> exp_sepcon2. iExists rp2. rewrite -> exp_sepcon2. iExists (Some (k1,v3,g11,g12)). simpl. 
+        rewrite <- !sepcon_assoc.   rewrite -> exp_sepcon2. iExists sh4.  
+         rewrite (prop_true_andp _ (ghost_snap (n3, n4, Some (k1, v3, g11, g12)) g1)). 
+        rewrite (prop_true_andp ( readable_share sh4 ∧ (Int.min_signed ≤ k1 ∧ k1 ≤ Int.max_signed)∧ is_pointer_or_null lp2 ∧ is_pointer_or_null rp2 /\  is_pointer_or_null v3  ) _ ).
+       destruct H15. rewrite H14.  iFrame .
+       iApply "Tclose". 
+       iFrame.
+       iSplit. iPureIntro;auto.
+       unfold tree_rep2.
+       iExists tg.
+       iFrame;iSplit;auto.
+       iApply "Tree".
+       unfold node_information, node_data. rewrite -> exp_sepcon2.  iExists sh5.
+       iFrame. iSplit. iPureIntro;auto. auto. destruct H15;split; auto. auto. auto.
+     }
+    Intros tp2.
+    if_tac. 
+     { gather_SEP ( in_tree g1 (n1, Finite_Integer k) lp1 g).
+        viewshift_SEP 0 (emp). 
+         { go_lower. unfold in_tree, ghost_snap, ghost_part. Intros sh'.  iIntros "H"; iMod (own_dealloc with "H");eauto. }
+        forward. 
+        Exists (lp1,tp2,g1). if_tac. unfold nodebox_rep. Intros tp3 lp3.  Exists tp3 (tp0::lp3) . simpl iter_sepcon. Exists sh1. entailer!. admit.  (* extra AS && cored, need to fix*)
+      simpl in H9;contradiction H9.
+      }
+    Intros n3 n4 lp2 rp2 info2. 
+    forward.   Exists (lp1,tp2,g1). if_tac. contradiction H8. Exists n3 n4 n1 (Finite_Integer k) info2 lp2 rp2.  unfold nodebox_rep. Intros tp3 lp3. Exists tp3 (tp0::lp3). simpl iter_sepcon. Exists sh1. entailer!.  
+    { unfold check_key_exist', range_inclusion in *. apply andb_true_intro. apply andb_prop in H9.  apply andb_prop in H1. destruct H1, H9. split.
+      apply less_than_equal_less_than_transitivity with (b := n1);auto. apply less_than_less_than_equal_transitivity with  (b := Finite_Integer k);auto. simpl. apply Zaux.Zlt_bool_true ;auto.
+    }  cancel. 
+  **   forward. (* second else if, then clause: x<y *)
+    sep_apply (in_tree_split g2 ( Finite_Integer k,n2) rp g).
+    sep_apply cored_dup.
+    forward_call (rp, top, empty, fun tp : val => if eq_dec tp nullval then  Q nullval else |> P * EX n n0:number, EX lp:val, EX rp:val, EX info: option ghost_info, !!(range_inclusion ( Finite_Integer k,n2) (n,n0) = true) && ghost_snap (n, n0,info) g2 * node_data_without_value info g tp lp rp  (n,n0) , inv_names).
+    { subst Frame;instantiate (1 := [ AS && cored ; in_tree g2 (Finite_Integer k,n2) rp g; mem_mgr gv; data_at sh1 t_struct_tree (vint k, (vp, (lp1, rp))) tp0; nodebox_rep sh b g_root g]).  simpl;cancel.
+      iIntros "((((( [AS1 _] & in1) & in2) & P ) & snap) & in)". 
+      iMod ("AS1" with "P") as (BST) "[Tree Tclose]". 
+      iDestruct "Tree" as "(% & Tree)".
+      unfold tree_rep2 at 1.
+      iDestruct "Tree" as (tg) "((% & Tree) & gref)".
+      iPoseProof (node_exist_in_tree with "[gref in1]") as "%". iFrame. destruct H11 as [r H11]. destruct r as [n3 n4]. destruct H11.
+      iPoseProof ( extract_left_node_info_from_ghost_tree_rep with "Tree") as "Hadd". apply H11. intros. simpl;auto.
+      iDestruct "Hadd" as ( tp2 o lp2 rp2 v) "(info & Tree)". 
+      unfold node_information at 1.
+      iDestruct "info" as "(% &((p & master) & info))". 
+       iModIntro; iExists Ews, tp2. iFrame "p".
+       iSplitL ""; [iSplit; auto; iPureIntro; split; auto; tauto|].
+        iIntros "p".
+        iPoseProof (make_snap with "[master]") as "master". iFrame.
+        iMod ("master") as "[snap1 master]". 
+        iDestruct "in" as (sh7) "in".
+       iMod (own_dealloc with "in") as "_".
+       iDestruct "in1" as (sh8) "in1".
+       iMod (own_dealloc with "in1") as "_". 
+        iDestruct "in2" as (sh2) "in2".
+       iMod (own_dealloc with "in2") as "_".
+        iMod (own_dealloc with "snap") as "_".
+       rewrite  node_data_R. unfold node_data_without_value. 
+       assert ( check_key_exist' x (n3,n4) = true).
+       { unfold check_key_exist', range_inclusion in *. apply andb_true_intro. apply andb_prop in H1. apply andb_prop in H12. destruct H1, H12. split.
+          apply less_than_equal_less_than_transitivity with (b :=  (Finite_Integer k) );auto. simpl. apply Zaux.Zlt_bool_true ;auto. apply less_than_less_than_equal_transitivity with  (b := n2);auto. 
+        }  
+       destruct (eq_dec tp2 nullval).
+       * iMod (own_dealloc with "snap1") as "_". iDestruct "Tclose" as "[_ Tclose]".
+         iSpecialize ("Tclose" $! nullval). iApply "Tclose". iDestruct "info" as "(% & _)".
+         rewrite prop_true_andp.
+         unfold tree_rep2.
+          rewrite -> exp_sepcon1.  
+         iExists tg.
+         iFrame;iSplit;auto.
+         iApply "Tree".
+         unfold node_information, node_data. destruct H15. rewrite H15. iFrame. iPureIntro. split;auto.
+         split;auto. symmetry. apply lookup_not_in. destruct H15. rewrite  H15 in H13. destruct H16. destruct H17. rewrite H18 in H13.  eapply range_info_in_tree_not_In in H13.  rewrite <- H10. apply H13. rewrite <-H10 in H9;auto. auto. intros;auto. 
+        * 
+          iDestruct "Tclose" as "[Tclose _]".    iDestruct "info" as (g0 sh3) "info".  destruct g0 as [[[k1 v3] g11 ] g12].  iDestruct "info" as "(((((% & v) & malloc ) & tp) & g1) & g2)". simpl in *.
+         destruct H15. apply split_readable_share in H15. destruct H15 as (sh4 & sh5 & H18 & H17 & H19). rewrite <- (data_at_share_join sh4 sh5 sh3 _ _ _). iDestruct "tp" as "(tp1 & tp2)".
+          rewrite (in_tree_split g11 ( n3, Finite_Integer k1) lp2 g). rewrite ( in_tree_split g12 ( Finite_Integer k1, n4) rp2 g ). iDestruct "g1" as "(g11 & g12)". iDestruct "g2" as "(g21 & g22)".
+        rewrite -> exp_sepcon2.  iExists n3.  rewrite -> exp_sepcon2.  iExists n4.  rewrite -> exp_sepcon2.  iExists lp2. rewrite -> exp_sepcon2. iExists rp2. rewrite -> exp_sepcon2. iExists (Some (k1,v3,g11,g12)). simpl. 
+        rewrite <- !sepcon_assoc.   rewrite -> exp_sepcon2. iExists sh4.  
+         rewrite (prop_true_andp _ (ghost_snap (n3, n4, Some (k1, v3, g11, g12)) g2)). 
+        rewrite (prop_true_andp ( readable_share sh4 ∧ (Int.min_signed ≤ k1 ∧ k1 ≤ Int.max_signed)∧ is_pointer_or_null lp2 ∧ is_pointer_or_null rp2 /\  is_pointer_or_null v3  ) _ ).
+       destruct H16. rewrite H15.  iFrame .
+       iApply "Tclose". 
+       iFrame.
+       iSplit. iPureIntro;auto.
+       unfold tree_rep2.
+       iExists tg.
+       iFrame;iSplit;auto.
+       iApply "Tree".
+       unfold node_information, node_data. rewrite -> exp_sepcon2.  iExists sh5.
+       iFrame. iSplit. iPureIntro;auto. auto. destruct H16;split; auto. auto. auto.
+     }
+    Intros tp2.
+    if_tac. 
+     { gather_SEP ( in_tree g2 ( Finite_Integer k,n2) rp g).
+        viewshift_SEP 0 (emp). 
+         { go_lower. unfold in_tree, ghost_snap, ghost_part. Intros sh'.  iIntros "H"; iMod (own_dealloc with "H");eauto. }
+        forward. 
+        Exists (rp,tp2,g2). if_tac. unfold nodebox_rep. Intros tp3 lp3.  Exists tp3 (tp0::lp3) . simpl iter_sepcon. Exists sh1. entailer!. admit.  (* extra AS && cored, need to fix*)
+      simpl in H9;contradiction H9.
+      }
+    Intros n3 n4 lp2 rp2 info2. 
+    forward.   Exists (rp,tp2,g2). if_tac. contradiction H9. Exists n3 n4  (Finite_Integer k) n2 info2 lp2 rp2.  unfold nodebox_rep. Intros tp3 lp3. Exists tp3 (tp0::lp3). simpl iter_sepcon. Exists sh1. entailer!.  
+    { unfold check_key_exist', range_inclusion in *. apply andb_true_intro. apply andb_prop in H10.  apply andb_prop in H1. destruct H1, H10. split.
+      apply less_than_equal_less_than_transitivity with (b := (Finite_Integer k));auto.  simpl. apply Zaux.Zlt_bool_true ;auto. apply less_than_less_than_equal_transitivity with  (b :=n2);auto. 
+    }  cancel. 
+    
+ ** forward. (* else clause  : x = k *)
+     focus_SEP 6.
+     forward_call (vp, top, empty, fun v:val => Q v, inv_names).
+    { subst Frame;instantiate (1 := [data_at sh1 t_struct_tree (vint k, (vp, (lp1, rp))) tp0;mem_mgr gv;nodebox_rep sh b g_root g]).  simpl;cancel.
+      iIntros "((((( [AS1 _] & in1) & in2) & P ) & snap) & in)". 
+      iMod ("AS1" with "P") as (BST) "[Tree Tclose]". 
+      iDestruct "Tree" as "(% & Tree)".
+      unfold tree_rep2 at 1.
+      iDestruct "Tree" as (tg) "((% & Tree) & gref)".
+      iPoseProof (node_exist_in_tree with "[gref in]") as "%". iFrame. destruct H11 as [r H11]. destruct r as [n3 n4]. destruct H11.
+      iPoseProof ( extract_left_node_info_from_ghost_tree_rep with "Tree") as "Hadd". apply H11. intros. simpl;auto.
+      iDestruct "Hadd" as ( tp2 o lp2 rp2 v) "(info & Tree)". 
+      unfold node_information at 1.
+      iDestruct "info" as "(% & ((p & master) & info))".
+       iCombine "snap master" as "master"; rewrite -> snap_master_join1. 
+       iDestruct "master" as "[ % master]".
+       destruct H14.  rewrite H4 in H15. simpl in H15.  rewrite <- H15. unfold node_data. 
+       iDestruct "info" as (sh4) "(((((% & vp) & token ) & tp ) & in11 ) & in21)".
+       unfold in_tree, ghost_part at 1. unfold in_tree, ghost_part at 1. unfold in_tree, ghost_part at 1.
+       iDestruct "in1" as (sh8) "in1". iMod (own_dealloc with "in1") as "_".
+        iDestruct "in2" as (sh9) "in2". iMod (own_dealloc with "in2") as "_".
+       iDestruct "in" as (sh10) "in". iMod (own_dealloc with "in") as "_".
+       iModIntro. iExists Ews. iExists v.  iFrame "vp".
+       iSplitL ""; [iSplit; auto; iPureIntro; split; auto; tauto|].
+        iIntros "np".
+       iDestruct "Tclose" as "[_ Tclose ]".
+       iSpecialize ("Tclose" $! v).
+       iApply ("Tclose"). rewrite <- H10 in H9. assert (k = x). { omega. } rewrite H17 in H15. rewrite <- H15 in H13.
+       apply (sorted_tree_look_up_in x v vp g1 g2 tg _ _ H9) in H13.
+       rewrite prop_true_andp. unfold tree_rep2.
+       rewrite -> exp_sepcon1. iExists tg.
+       iFrame;iSplit;auto.
+       iApply "Tree".
+       unfold node_information, node_data. rewrite -> exp_sepcon2.  iExists sh4.
+       iFrame. iSplit. iPureIntro;auto. auto. split. rewrite <-H10;auto. rewrite <-H10;auto.
+     }
+     Intros v.
+     forward.
+     forward.
+     Exists v.
+     unfold nodebox_rep. Intros tp3 lp3. Exists tp3 (tp0::lp3). simpl iter_sepcon. Exists sh1. entailer!.
+* (* After the loop *) 
+  if_tac. forward. Exists nullval.  entailer!.  contradiction HRE.  
+Admitted.
 
 Lemma body_insert: semax_body Vprog Gprog f_insert insert_spec.
 Proof.
@@ -85,7 +373,7 @@ forward.
     | apply (semax_loop _ (insert_inv b sh x v g_root gv g inv_names P AS ref) (insert_inv b sh x v g_root gv g inv_names P AS ref) )]. 
 
 * (* Precondition *) 
-   intros. unfold insert_inv.  Exists b g_root.  unfold nodebox_rep in *. Intros tp lp. Exists Neg_Infinity Pos_Infinity tp lp. sep_apply (in_tree_split g_root ( Neg_Infinity, Pos_Infinity) b g) . entailer!.
+   intros. unfold insert_inv.  Exists b g_root.  unfold nodebox_rep in *.  Intros tp lp. Exists Neg_Infinity Pos_Infinity tp lp. sep_apply (in_tree_split g_root ( Neg_Infinity, Pos_Infinity) b g) . entailer!.
 
 *  (* Loop body *)
    unfold insert_inv. Intros np g_current n1 n2. 
@@ -140,7 +428,7 @@ forward.
          iExists tg.
          iFrame;iSplit;auto.
          iApply "Tree".
-         unfold node_information, node_data. iFrame. iPureIntro. split. apply H7. auto. apply H7.
+         unfold node_information, node_data. iFrame. iPureIntro. split. apply H7. auto. destruct H7. destruct H8.  destruct H9. split;auto. 
          unfold range_inclusion, check_key_exist' in *.  apply andb_prop in H1. apply andb_prop in H5. destruct H1, H5. apply andb_true_intro. split. apply less_than_equal_less_than_transitivity with (b := n1). apply H5. apply H1. assert (less_than (Finite_Integer x) n0 = true). { apply less_than_less_than_equal_transitivity with (b := n2). apply H7. apply H8. } apply H9.
   } 
  Intro tp.
@@ -215,7 +503,7 @@ forward.
        apply less_than_less_than_equal_transitivity with  (b := n2). apply H16. apply H18. }     
        iSpecialize ("Tree" with "[rp1 lp1 v1 p token np lg inl rg inr master ]") . instantiate(1:= rp1).  instantiate(1:= lp1).   instantiate(1:= v1). 
        rewrite prop_true_andp. rewrite -> exp_sepcon2.  repeat rewrite exp_sepcon1.  iExists sh1. iFrame. iPureIntro. split;auto. destruct H17. repeat split;auto. destruct H. auto. destruct H;auto. 
-       destruct H17. repeat split;auto.
+       destruct H17. destruct H18.  repeat split;auto.
         iDestruct "Tree" as "(% & Tree)".
         rewrite prop_true_andp.  assert (H19 := H18). apply (key_not_exist_in_tree _ _ _ x) in H18.
        rewrite (update_ghost_tree_with_insert x v v1 tg gl gr g_root _ lp1 rp1 b n3 n4 None). iFrame. auto. apply H14. apply H15. apply H18.
